fstar

libcrux-ml-kem/src/ind_cca.rs
@@ -582,7 +582,12 @@ pub(crate) mod unpacked {
 
     /// Take a serialized private key and generate an unpacked key pair from it.
     #[inline(always)]
-    #[hax_lib::requires(fstar!("Spec.MLKEM.is_rank $K"))]
+    #[hax_lib::requires(fstar!("Spec.MLKEM.is_rank $K /\\
+           v_SECRET_KEY_SIZE == Spec.MLKEM.v_CCA_PRIVATE_KEY_SIZE v_K /\\
+           v_CPA_SECRET_KEY_SIZE == Spec.MLKEM.v_CPA_PRIVATE_KEY_SIZE v_K /\\
+           v_PUBLIC_KEY_SIZE == Spec.MLKEM.v_CPA_PUBLIC_KEY_SIZE v_K /\\
+           v_BYTES_PER_RING_ELEMENT == Spec.MLKEM.v_RANKED_BYTES_PER_RING_ELEMENT v_K /\\
+           v_T_AS_NTT_ENCODED_SIZE == Spec.MLKEM.v_T_AS_NTT_ENCODED_SIZE v_K)"))]
     pub fn keys_from_private_key<
         const K: usize,
         const SECRET_KEY_SIZE: usize,
@@ -641,6 +646,12 @@ pub(crate) mod unpacked {
 
         /// Take a serialized private key and generate an unpacked key pair from it.
         #[inline(always)]
+        #[requires(fstar!("Spec.MLKEM.is_rank $K /\\
+           v_SECRET_KEY_SIZE == Spec.MLKEM.v_CCA_PRIVATE_KEY_SIZE v_K /\\
+           v_CPA_SECRET_KEY_SIZE == Spec.MLKEM.v_CPA_PRIVATE_KEY_SIZE v_K /\\
+           v_PUBLIC_KEY_SIZE == Spec.MLKEM.v_CPA_PUBLIC_KEY_SIZE v_K /\\
+           v_BYTES_PER_RING_ELEMENT == Spec.MLKEM.v_RANKED_BYTES_PER_RING_ELEMENT v_K /\\
+           v_T_AS_NTT_ENCODED_SIZE == Spec.MLKEM.v_T_AS_NTT_ENCODED_SIZE v_K)"))]
         pub fn from_private_key<
             const SECRET_KEY_SIZE: usize,
             const CPA_SECRET_KEY_SIZE: usize,
