libcrux-ml-kem/src/types.rs
@@ -203,6 +203,18 @@ impl<const PRIVATE_KEY_SIZE: usize, const PUBLIC_KEY_SIZE: usize>
 /// Unpack an incoming private key into it's different parts.
 ///
 /// We have this here in types to extract into a common core for C.
+#[hax_lib::requires(fstar!("Seq.length private_key >= 
+                            v v_CPA_SECRET_KEY_SIZE + v v_PUBLIC_KEY_SIZE + 
+                            v Libcrux_ml_kem.Constants.v_H_DIGEST_SIZE"))]
+#[hax_lib::ensures(|result| fstar!("
+           let (ind_cpa_secret_key,ind_cpa_public_key,ind_cpa_public_key_hash,implicit_rejection_value)
+               = result in
+           Seq.length ind_cpa_secret_key == v v_CPA_SECRET_KEY_SIZE /\\
+           Seq.length ind_cpa_public_key == v v_PUBLIC_KEY_SIZE /\\
+           Seq.length ind_cpa_public_key_hash == v Libcrux_ml_kem.Constants.v_H_DIGEST_SIZE /\\
+           Seq.length implicit_rejection_value == 
+           Seq.length private_key - 
+             (v v_CPA_SECRET_KEY_SIZE + v v_PUBLIC_KEY_SIZE + v Libcrux_ml_kem.Constants.v_H_DIGEST_SIZE)"))]
 pub(crate) fn unpack_private_key<const CPA_SECRET_KEY_SIZE: usize, const PUBLIC_KEY_SIZE: usize>(
     private_key: &[u8], // len: SECRET_KEY_SIZE
 ) -> (&[u8], &[u8], &[u8], &[u8]) {
